syn/ex/Mesi/MesiComp.v
@@ -13,18 +13,40 @@ Section Tests.
   Definition dln: string := "DownLock".
   Definition ostin: string := "ost".
 
-  Context `{cet: @CompExtType DirExtType}
-          `{@CompExtExp MesiHConfig
-                        SpecInds.NatDecValue
-                        Mesi.ImplOStateIfc
-                        DirExtType
-                        DirExtExp
-                        cet}.
+  Definition KMesi: Kind := Bit 3.
+  Definition KDir :=
+    STRUCT { "dir_st" :: KMesi;
+             "dir_excl" :: KIdxQ;
+             "dir_sharers" :: Array KIdxQ (Nat.pow 2 hcfg_children_max_lg) }.
 
+  Instance MesiCompExtType: CompExtType :=
+    {| kind_of_hetype :=
+         fun het => match het with
+                    | HDir => Struct KDir
+                    end
+    |}.
+
+  Instance MesiCompExtExp: CompExtExp :=
+    {| compile_eexp :=
+         fun var het ostVars he =>
+           match he in (hexp_dir _ h) return (kind_of h) @ (var) with
+           | HDirC _ =>
+             #(HVector.hvec_ith ostVars (Fin.FS (Fin.FS (Fin.FS Fin.F1))))
+           | HDirGet _ _ => TODO _
+           end%kami_expr
+    |}.
+
+  (* Opaque icons'. *)
   Existing Instance MesiHOStateIfcFull.
   Definition cl1GetSImm := compile_Rule oidx uln dln ostin (existT _ _ (hl1GetSImm oidx)).
   Goal True.
     pose cl1GetSImm as r.
+    compute in r.
+  Abort.
+
+  Definition cl1GetSRqUpUp := compile_Rule oidx uln dln ostin (existT _ _ (hl1GetSRqUpUp oidx)).
+  Goal True.
+    pose cl1GetSRqUpUp as r.
     compute in r.
   Abort.
 
